platform/cito/optimizers/ElimDead.v
@@ -1,99 +1,28 @@
+Set Implicit Arguments.
+
 Require Import Syntax.
 Import String Memory IL SyntaxExpr.
 Require Import Notations.
-Require Import Equalities SetModule.
 Require Import Semantics.
 Require Import GeneralTactics.
 Import SemanticsExpr.
 
-Set Implicit Arguments.
+Require Import Equalities.
+Require Import StringSet.
+Module Import SS := StringSet.
+Require Import SetFacts.
+Require Import FSetFacts1.
+Module SK_as_UDT := Make_UDT StringKey.
+Require Import FSetFacts1.
+Module Import SF1 := UWFacts_fun SK_as_UDT SS.
+Import P FM.
 
-Module Key <: MiniDecidableType.
-  Definition t := string.
-  Definition eq_dec := string_dec.
-End Key.
-
-Module MSet := ArrowSet Key.
-Import MSet.
-
-Notation skip := Syntax.Skip.
-Notation free := Syntax.Free.
-Notation len := Syntax.Len.
-Notation eval := exprDenote.
-
-Open Scope stmnt.
-Open Scope set.
-
-Fixpoint used_vars e :=
-  match e with
-    | Const _ => 0
-    | Var x => !x
-    | Binop _ a b => used_vars a + used_vars b
-    | TestE _ a b => used_vars a + used_vars b
-  end.
-
-Fixpoint used_vars_stmt s :=
-  match s with
-    | skip => 0
-    | a ;;; b => used_vars_stmt a + used_vars_stmt b
-    | Conditional e t f => used_vars e + used_vars_stmt t + used_vars_stmt f
-    | Loop e body => used_vars e + used_vars_stmt body
-    | x <- e => used_vars e
-    | x <== arr[idx] => used_vars arr + used_vars idx
-    | arr[idx] <== e => used_vars arr + used_vars idx + used_vars e
-    | x <- new e => used_vars e
-    | free e => used_vars e
-    | len x e => used_vars e
-    | Call f[x] => used_vars f + used_vars x
-  end.
-
-Fixpoint elim_dead s used : Statement * set :=
-  match s with
-    | skip => (s, used)
-    | a ;;; b => 
-      let result := elim_dead b used in
-      let b := fst result in
-      let used := snd result in
-      let result := elim_dead a used in
-      let a := fst result in
-      let used := snd result in
-      (a ;;; b, used)
-    | Conditional e t f => 
-      let result := elim_dead t used in
-      let t := fst result in
-      let used_t := snd result in
-      let result := elim_dead f used in
-      let f := fst result in
-      let used_f := snd result in
-      (Conditional e t f, used_vars e + used_t + used_f)
-    | Loop e body => 
-      let result := elim_dead body (used + used_vars e + used_vars_stmt body) in
-      let body := fst result in
-      let used' := snd result in
-      (Loop e body, used + used' + used_vars e)
-    | x <- e =>
-      if mem_dec x used then
-        (s, used - !x + used_vars e)
-      else
-        (skip, used)
-    | x <== arr[idx] =>
-      (s, used - !x + used_vars arr + used_vars idx)
-    | arr[idx] <== e =>
-      (s, used + used_vars arr + used_vars idx + used_vars e)
-    | x <- new e =>
-      (s, used - !x + used_vars e)
-    | free e =>
-      (s, used + used_vars e)
-    | len x e =>
-      (s, used - !x + used_vars e)
-    | Call f[x] =>
-      (s, used + used_vars f + used_vars x)
-  end.
+Definition SET := SS.t.
 
 Ltac openhyp' :=
   repeat match goal with
-           | H : context [mem_dec ?A ?B] |- _ => destruct (mem_dec A B)
-           | |- context [mem_dec ?A ?B] => destruct (mem_dec A B)
+           | H : context [In_dec ?A ?B] |- _ => destruct (In_dec A B)
+           | |- context [In_dec ?A ?B] => destruct (In_dec A B)
            | H : context [ { _ | _ } ] |- _ => destruct H
          end.
 
@@ -102,488 +31,631 @@ Ltac unfold_all :=
            | H := _ |- _ => unfold H in *; clear H
          end.
 
-Open Scope set_scope.
-
-Ltac subset_solver :=
-  repeat 
-    match goal with
-      | |- ?A <= ?A => eapply subset_refl
-      | |- _ + _ <= _ => eapply union_subset
-      | |- ?S <= ?A + _ =>
-        match A with
-            context [ S ] => eapply subset_trans; [ .. | eapply subset_union_left]
-        end
-      | |- ?S <= _ + ?B =>
-        match B with
-            context [ S ] => eapply subset_trans; [ .. | eapply subset_union_right]
-        end
-      | |- _ - _ <= _ => eapply subset_trans; [ eapply diff_subset | .. ]
-      end.
-
-Hint Extern 0 (subset _ _) => progress subset_solver.
-
-Definition agree_in a b s := forall x, x ^ s -> Locals.sel a x = Locals.sel b x.
-
-Lemma agree_in_symm : forall a b s, agree_in a b s -> agree_in b a s.
-  unfold agree_in; intros; symmetry; eauto.
-Qed.
-
-Lemma agree_in_subset : forall a b s s', agree_in a b s -> (s' <= s)%set -> agree_in a b s'.
-  unfold agree_in; intros; eapply subset_correct in H0; eauto.
-Qed.
-
-Lemma upd_same_agree_in : forall a b s x w, agree_in a b (s - !x) -> agree_in (upd a x w) (upd b x w) s.
-  unfold agree_in; intros.
-  destruct (string_dec x x0).
-  subst.
-  repeat rewrite sel_upd_eq; eauto.
-  repeat rewrite sel_upd_ne; eauto.
-  eapply H.
-  eapply diff_correct.
-  intuition.
-  eapply singleton_correct in H1.
-  intuition.
-Qed.
-
-Lemma upd_out_agree_in : forall a b s x w, agree_in a b s -> ~ x ^ s -> agree_in (upd a x w) b s.
-  unfold agree_in; intros.
-  destruct (string_dec x x0).
-  subst; intuition.
-  repeat rewrite sel_upd_ne; eauto.
-Qed.
-
-Hint Constructors RunsTo.
-Hint Resolve upd_same_agree_in.
-Hint Resolve agree_in_subset.
-Hint Resolve upd_out_agree_in.
-Hint Resolve agree_in_symm.
-Hint Resolve subset_union_left subset_union_right.
-
-Lemma elim_dead_upper_bound : 
-  forall s used,
-    let result := elim_dead s used in
-    let used' := snd result in
-    used' <= used + used_vars_stmt s.
-Proof.
-  induction s; simpl; intuition eauto using subset_trans.
-  openhyp'; simpl in *; eauto.
-Qed.
-Hint Resolve elim_dead_upper_bound.
-
 Ltac f_equal' :=
   match goal with
     | |- (if ?E1 then _ else _) = (if ?E2 then _ else _) => replace E2 with E1; try reflexivity
   end.
 
-Lemma eval_agree_in : forall e a b, agree_in a b (used_vars e) -> eval e a = eval e b.
-  induction e; simpl; intuition.
-  eapply H; eapply singleton_correct; eauto.
-  f_equal; eauto.
-  f_equal'; f_equal; eauto.
-Qed.
+Section TopSection.
 
-Lemma while_case :
-  forall fs t v v',
-    RunsTo fs t v v' ->
-    forall e body used vs,
-      let s := Loop e body in
+  Notation "m %%- k" := (remove k m) (at level 60).
+  Infix "<=" := Subset : set_scope.
+  Infix "+" := union.
+  Infix "-" := diff.
+  Notation "! x" := (singleton x) (at level 40).
+  Notation "[]" := (@empty _).
+  Open Scope set_scope.
+  Open Scope stmt_scope.
+  Infix "<-" := Syntax.Assign.
+
+  Fixpoint used_vars e :=
+    match e with
+      | Const _ => empty
+      | Var x => !x
+      | Binop _ a b => used_vars a + used_vars b
+      | TestE _ a b => used_vars a + used_vars b
+    end.
+
+  Require Import Union.
+
+  Fixpoint used_vars_stmt s :=
+    match s with
+      | skip => empty
+      | a ;; b => used_vars_stmt a + used_vars_stmt b
+      | Syntax.If e t f => used_vars e + used_vars_stmt t + used_vars_stmt f
+      | Syntax.While e body => used_vars e + used_vars_stmt body
+      | _ <- e => used_vars e
+      | Syntax.Label _ _ => empty
+      | Syntax.Call _ f args => used_vars f + union_list (List.map used_vars args)
+    end.
+
+  Require Import Option.
+
+  Fixpoint elim_dead s used : Stmt * SET :=
+    match s with
+      | skip => (s, used)
+      | a ;; b => 
+        let result := elim_dead b used in
+        let b := fst result in
+        let used := snd result in
+        let result := elim_dead a used in
+        let a := fst result in
+        let used := snd result in
+        (a ;; b, used)
+      | Syntax.If e t f => 
+        let result := elim_dead t used in
+        let t := fst result in
+        let used_t := snd result in
+        let result := elim_dead f used in
+        let f := fst result in
+        let used_f := snd result in
+        (Syntax.If e t f, used_vars e + used_t + used_f)
+      | Syntax.While e body => 
+        let result := elim_dead body (used + used_vars e + used_vars_stmt body) in
+        let body := fst result in
+        let used' := snd result in
+        (Syntax.While e body, used + used' + used_vars e)
+      | x <- e =>
+        if In_dec x used then
+          (s, used - !x + used_vars e)
+        else
+          (skip, used)
+      | Syntax.Label x _ =>
+        (s, used - !x)
+      | Syntax.Call x f args =>
+        (s, used - (default empty (option_map singleton x)) + used_vars f + union_list (List.map used_vars args))
+    end.
+
+  Hint Extern 0 (Subset _ _) => progress (simpl; subset_solver).
+  Hint Resolve subset_union_left subset_union_right.
+  Hint Resolve diff_subset.
+
+  Definition agree_in a b s := forall x, In x s -> Locals.sel a x = Locals.sel b x.
+
+  Lemma agree_in_symm : forall a b s, agree_in a b s -> agree_in b a s.
+    unfold agree_in; intros; symmetry; eauto.
+  Qed.
+
+  Hint Resolve agree_in_symm.
+
+  Lemma agree_in_subset : forall a b s s', agree_in a b s -> s' <= s -> agree_in a b s'.
+    unfold agree_in, Subset; intros; eauto.
+  Qed.
+
+  Hint Resolve agree_in_subset.
+
+  Require Import GeneralTactics2.
+
+  Lemma upd_same_agree_in : forall a b s x w, agree_in a b (s - !x) -> agree_in (upd a x w) (upd b x w) s.
+    unfold agree_in; intros.
+    destruct (string_dec x x0).
+    subst.
+    repeat rewrite sel_upd_eq; eauto.
+    repeat rewrite sel_upd_ne.
+    eapply H; eauto.
+    eapply diff_iff.
+    split; eauto.
+    not_not.
+    eapply singleton_iff in H1; eauto.
+    eauto.
+    eauto.
+  Qed.
+
+  Hint Resolve upd_same_agree_in.
+
+  Lemma upd_out_agree_in : forall a b s x w, agree_in a b s -> ~ In x s -> agree_in (upd a x w) b s.
+    unfold agree_in; intros.
+    destruct (string_dec x x0).
+    subst; intuition.
+    repeat rewrite sel_upd_ne; eauto.
+  Qed.
+
+  Hint Resolve upd_out_agree_in.
+
+  Lemma elim_dead_upper_bound : 
+    forall s used,
       let result := elim_dead s used in
-      let s' := fst result in
       let used' := snd result in
-      let vt := fst v in
-      let heap := snd v in
-      let vt' := fst v' in
-      let heap' := snd v' in
-      t = s' ->
-      agree_in vs vt used' ->
-      (
-        let s := body in
+      used' <= used + used_vars_stmt s.
+  Proof.
+    induction s; simpl; intros; openhyp'; intuition eauto using subset_trans.
+    Grab Existential Variables.
+    eapply empty.
+  Qed.
 
-        forall (used : set) (vs vt : vals) (heap : arrays) 
-               (vt' : vals) (heap' : arrays),
+  Hint Resolve elim_dead_upper_bound.
+
+  Lemma eval_agree_in : forall e a b, agree_in a b (used_vars e) -> eval a e = eval b e.
+    induction e; simpl; intuition.
+    eapply H; eapply singleton_iff; eauto.
+    f_equal; eauto.
+    f_equal'; f_equal; eauto.
+  Qed.
+
+  Lemma eval_agree_in_list : forall es a b, agree_in a b (union_list (List.map used_vars es)) -> List.map (eval a) es = List.map (eval b) es.
+    induction es; simpl; intuition.
+    f_equal.
+    eapply eval_agree_in; eauto.
+    eauto.
+  Qed.
+
+End TopSection.
+
+Require Import ADT.
+
+Module Make (Import E : ADT).
+
+  Require Import GoodOptimizer.
+  Module Import GoodOptimizerMake := GoodOptimizer.Make E.
+  Require Import Semantics.
+  Import SemanticsMake.
+
+  Section TopSection.
+
+    Hint Unfold RunsTo.
+    Hint Constructors Semantics.RunsTo.
+    Hint Unfold Safe.
+    Hint Constructors Semantics.Safe.
+
+    Notation "m %%- k" := (remove k m) (at level 60).
+    Infix "<=" := Subset : set_scope.
+    Infix "+" := union.
+    Infix "-" := diff.
+    Notation "! x" := (singleton x) (at level 40).
+    Notation "[]" := (@empty _).
+    Open Scope set_scope.
+    Open Scope stmt_scope.
+    Infix "<-" := Syntax.Assign.
+
+    Hint Extern 0 (Subset _ _) => progress (simpl; subset_solver).
+    Hint Resolve subset_union_left subset_union_right.
+    Hint Resolve diff_subset.
+    Hint Resolve agree_in_symm.
+    Hint Resolve agree_in_subset.
+    Hint Resolve upd_same_agree_in.
+    Hint Resolve upd_out_agree_in.
+    Hint Resolve elim_dead_upper_bound.
+
+    Lemma while_case :
+      forall fs t v v',
+        RunsTo fs t v v' ->
+        forall e body used vs,
+          let s := Syntax.While e body in
           let result := elim_dead s used in
-          let t := fst result in
+          let s' := fst result in
           let used' := snd result in
-          RunsTo fs t (vt, heap) (vt', heap') ->
+          let vt := fst v in
+          let heap := snd v in
+          let vt' := fst v' in
+          let heap' := snd v' in
+          t = s' ->
           agree_in vs vt used' ->
-          exists vs' : vals,
-            RunsTo fs s (vs, heap) (vs', heap') /\ agree_in vs' vt' used
-      ) ->
-      exists vs',
-        RunsTo fs s (vs, heap) (vs', heap') /\
-        agree_in vs' vt' used.
-Proof.
-  induction 1; simpl; intros; unfold_all; subst; intuition.
-
-  injection H2; intros; subst.
-  destruct v; simpl in *.
-  destruct v'; simpl in *.
-  eapply H4 in H0; eauto; openhyp.
-  destruct v''; simpl in *.
-  edestruct IHRunsTo2; try reflexivity.
-  2 : eauto.
-  eauto using subset_trans.
-  openhyp.
-  descend.
-  econstructor.
-  simpl. 
-  repeat erewrite (@eval_agree_in _ vs w) by eauto.
-  eauto.
-  eauto.
-  eauto.
-  eauto.
-
-  injection H0; intros; subst.
-  descend.
-  econstructor 9.
-  simpl.
-  repeat erewrite (@eval_agree_in _ vs (fst v)) by eauto.
-  eauto.
-  eauto.
-Qed.
-
-Lemma elim_dead_is_bp : 
-  forall fs s used vs vt heap vt' heap', 
-    let result := elim_dead s used in
-    let t := fst result in
-    let used' := snd result in
-    RunsTo fs t (vt, heap) (vt', heap') ->
-    agree_in vs vt used' ->
-    exists vs',
-      RunsTo fs s (vs, heap) (vs', heap') /\
-      agree_in vs' vt' used.
-Proof.
-  induction s; simpl; intros.
-
-  openhyp'; simpl in *.
-  inversion H; unfold_all; subst.
-  descend; intuition.
-  erewrite eval_agree_in by eauto.
-  eauto.
-
-  inversion H; unfold_all; subst.
-  descend; intuition.
-
-  inversion H; unfold_all; subst.
-  descend.
-  econstructor.
-  repeat erewrite (@eval_agree_in _ vs vt) by eauto.
-  eauto.
-  repeat erewrite (@eval_agree_in _ vs vt) by eauto.
-  eauto.
-
-  inversion H; unfold_all; subst.
-  descend; intuition.
-  repeat erewrite (@eval_agree_in _ vt' vs) by eauto.
-  econstructor.
-  repeat erewrite (@eval_agree_in _ vs vt') by eauto.
-  eauto.
-  eauto.
-  
-  inversion H; unfold_all; subst.
-  destruct v'; simpl in *.
-  eapply IHs1 in H3; eauto; openhyp.
-  eapply IHs2 in H6; eauto; openhyp.
-  descend.
-  eauto.
-  eauto.
-
-  inversion H; unfold_all; subst.
-  descend.
-  eauto.
-  eauto.
-
-  inversion H; unfold_all; subst.
-  simpl in *.
-  eapply IHs1 in H7; eauto; openhyp.
-  descend.
-  econstructor.
-  simpl.
-  repeat erewrite (@eval_agree_in _ vs vt) by eauto.
-  eauto.
-  eauto.
-  eauto.
-
-  simpl in *.
-  eapply IHs2 in H7; eauto; openhyp.
-  descend.
-  econstructor 7.
-  simpl.
-  repeat erewrite (@eval_agree_in _ vs vt) by eauto.
-  eauto.
-  eauto.
-  eauto.
-
-  eapply while_case in H; eauto.
-
-  inversion H; unfold_all; subst.
-  descend.
-  econstructor.
-  eauto.
-  repeat erewrite (@eval_agree_in _ vs vt) by eauto.
-  eauto.
-  repeat erewrite (@eval_agree_in _ vs vt) by eauto.
-  eauto.
-  eauto.
-
-  inversion H; unfold_all; subst.
-  descend.
-  repeat erewrite (@eval_agree_in _ vt' vs) by eauto.
-  econstructor.
-  repeat erewrite (@eval_agree_in _ vs vt') by eauto.
-  eauto.
-  eauto.
-
-  inversion H; unfold_all; subst.
-  descend.
-  econstructor.
-  repeat erewrite (@eval_agree_in _ vs vt) by eauto.
-  eauto.
-  repeat erewrite (@eval_agree_in _ vs vt) by eauto.
-  eauto.
-
-  inversion H; unfold_all; subst.
-  descend.
-  econstructor.
-  repeat erewrite (@eval_agree_in _ vs vt') by eauto.
-  eauto.
-  repeat erewrite (@eval_agree_in _ vs vt') by eauto.
-  eauto.
-  repeat erewrite (@eval_agree_in _ vs vt') by eauto.
-  eauto.
-  eauto.
-
-  descend.
-  econstructor 14.
-  repeat erewrite (@eval_agree_in _ vs vt') by eauto.
-  eauto.
-  repeat erewrite (@eval_agree_in _ vs vt') by eauto.
-  eauto.
-  eauto.
-  eauto.
-
-Qed.
-
-Import Safety.
-
-Hint Constructors Safe.
-
-Lemma elim_dead_is_sp :
-  forall fs s used vs vt heap,
-    let result := elim_dead s used in
-    let t := fst result in
-    let used' := snd result in
-    Safe fs s (vs, heap) ->
-    agree_in vs vt used' ->
-    Safe fs t (vt, heap).
-Proof.
-  induction s.
-
-  Focus 7.
-  intros.
-  unfold_all.
-  eapply 
-    (Safe_coind 
-       (fun t v =>
-          (exists vs c b used,
-             let s := While (c) {{b}} in
-             let result := elim_dead s used in
-             let s' := fst result in
-             let used' := snd result in
-             let vt := fst v in
-             let heap := snd v in
-             Safe fs s (vs, heap) /\
-             agree_in vs vt used' /\
-             (let s := b in
-              forall (used : set) (vs vt : vals) (heap : arrays),
-                Safe fs s (vs, heap) ->
-                agree_in vs vt (snd (elim_dead s used)) ->
-                Safe fs (fst (elim_dead s used)) (vt, heap)
-             ) /\
-             t = s') \/
-          Safe fs t v
-    )); [ .. | left; descend; simpl in *; intuition eauto ]; clear; simpl; intros; openhyp.
-
-  intuition.
-
-  inversion H; unfold_all; subst; eauto.
-
-  intuition.
-
-  inversion H; unfold_all; subst; eauto.
-
-  intuition.
-
-  inversion H; unfold_all; subst; intuition eauto.
-
-  intuition.
-
-  inversion H; subst.
-  intuition eauto.
-  right; intuition eauto.
-
-  injection H2; intros; subst.
-  inversion H; unfold_all; subst.
-  destruct v; simpl in *.
-  left.
-  repeat split.
-  repeat erewrite (@eval_agree_in _ v x) by eauto.
-  eauto.
-  eauto.
-
-  intros.
-  left.
-  destruct v'; simpl in *.
-  eapply elim_dead_is_bp in H3; eauto; openhyp.
-  descend.
-  4 : eauto.
-  eauto.
-  eauto using subset_trans.
-  eauto.
-
-  simpl in *.
-  right.
-  destruct v; simpl in *.
-  repeat erewrite (@eval_agree_in _ v x) by eauto.
-  eauto.
-
-  inversion H; unfold_all; subst.
-  intuition eauto.
-  right.
-  intuition eauto.
-
-  intuition.
-
-  inversion H; unfold_all; subst; eauto.
-
-  intuition.
-
-  inversion H; unfold_all; subst; eauto.
-
-  intuition.
-
-  inversion H; unfold_all; subst; eauto.
-
-  intuition.
-
-  inversion H; unfold_all; subst.
-  intuition eauto.
-  intuition eauto.
-
-  (* end of while case *)
-
-  simpl; intros; openhyp'; simpl in *; eauto.
-
-  simpl; intros.
-  inversion H; unfold_all; subst.
-  econstructor.
-  repeat erewrite (@eval_agree_in _ vt vs) by eauto.
-  eauto.
-  
-  simpl; intros.
-  inversion H; unfold_all; subst.
-  econstructor.
-  repeat erewrite (@eval_agree_in _ vt vs) by eauto.
-  eauto.
-  
-  simpl; intros.
-  inversion H; unfold_all; subst.
-  econstructor.
-  eauto.
-  intros.
-  destruct v'; simpl in *.
-  eapply elim_dead_is_bp in H1; eauto; openhyp.
-  eauto.
-
-  simpl; intros.
-  eauto.
-
-  simpl; intros.
-  inversion H; unfold_all; subst.
-  econstructor.
-  simpl in *.
-  repeat erewrite (@eval_agree_in _ vt vs) by eauto.
-  eauto.
-  eauto.
-
-  econstructor 5.
-  simpl in *.
-  repeat erewrite (@eval_agree_in _ vt vs) by eauto.
-  eauto.
-  eauto.
-
-  simpl; intros.
-  inversion H; unfold_all; subst.
-  econstructor.
-  repeat erewrite (@eval_agree_in _ vt vs) by eauto.
-  eauto.
-  
-  simpl; intros.
-  inversion H; unfold_all; subst.
-  econstructor.
-  repeat erewrite (@eval_agree_in _ vt vs) by eauto.
-  eauto.
-
-  simpl; intros.
-  inversion H; unfold_all; subst.
-  econstructor.
-  repeat erewrite (@eval_agree_in _ vt vs) by eauto.
-  eauto.
-
-  simpl; intros.
-  inversion H; unfold_all; subst.
-  econstructor.
-  repeat erewrite (@eval_agree_in _ vt vs) by eauto.
-  eauto.
-  repeat erewrite (@eval_agree_in _ vt vs) by eauto.
-  eauto.
-
-  econstructor 14.
-  repeat erewrite (@eval_agree_in _ vt vs) by eauto.
-  eauto.
-  repeat erewrite (@eval_agree_in _ vt vs) by eauto.
-  eauto.
-
-Qed.  
-
-Require Import SemanticsLemmas.
-Require Import CompileStatement.
-
-Lemma elim_dead_footprint : forall s m, List.incl (footprint (fst (elim_dead s m))) (footprint s).
-Proof.
-  induction s; simpl; intuition.
-  openhyp'; simpl in *; eauto.
-Qed.
-
-Open Scope nat.
-
-Lemma elim_dead_depth : forall s m, depth (fst (elim_dead s m)) <= depth s.
-Proof.
-  induction s; simpl; intuition.
-  openhyp'; simpl in *; eauto.
-Qed.
-
-Definition elim_dead_top s := fst (elim_dead s empty).
-
-Require Import GoodOptimizer.
-
-Lemma same_agree_in : forall a s, agree_in a a s.
-  unfold agree_in; intros; eauto.
-Qed.
-Hint Resolve same_agree_in.
-
-Lemma elim_dead_top_is_good_optimizer : is_good_optimizer elim_dead_top.
-  unfold is_good_optimizer, elim_dead_top.
-
-  descend.
-  destruct v; simpl in *.
-  eapply elim_dead_is_bp in H; eauto; openhyp.
-  descend; eauto.
-
-  destruct v; simpl in *.
-  eapply elim_dead_is_sp; eauto.
-
-  eapply elim_dead_footprint.
-
-  eapply elim_dead_depth.
-Qed.
+          (
+            let s := body in
+
+            forall (used : SET) (vs vt : vals) (heap : Heap) 
+                   (vt' : vals) (heap' : Heap),
+              let result := elim_dead s used in
+              let t := fst result in
+              let used' := snd result in
+              RunsTo fs t (vt, heap) (vt', heap') ->
+              agree_in vs vt used' ->
+              exists vs' : vals,
+                RunsTo fs s (vs, heap) (vs', heap') /\ agree_in vs' vt' used
+          ) ->
+          exists vs',
+            RunsTo fs s (vs, heap) (vs', heap') /\
+            agree_in vs' vt' used.
+    Proof.
+      induction 1; simpl; intros; unfold_all; subst; intuition.
+
+      injection H2; intros; subst.
+      destruct v; simpl in *.
+      destruct v'; simpl in *.
+      eapply H4 in H0; eauto; openhyp.
+      destruct v''; simpl in *.
+      edestruct IHRunsTo2; try reflexivity.
+      2 : eauto.
+      eauto using subset_trans.
+      openhyp.
+      descend.
+      econstructor.
+      simpl. 
+      repeat erewrite (@eval_agree_in _ vs w) by eauto.
+      eauto.
+      eauto.
+      eauto.
+      eauto.
+
+      injection H0; intros; subst.
+      descend.
+      eapply RunsToWhileFalse.
+      simpl.
+      repeat erewrite (@eval_agree_in _ vs (fst v)) by eauto.
+      eauto.
+      eauto.
+    Qed.
+
+    Lemma subset_diff_empty : forall s, s <= s - empty.
+      unfold Subset; intros.
+      eapply diff_iff; split; eauto.
+      nintro.
+      eapply empty_iff in H0; intuition.
+    Qed.
+
+    Hint Resolve subset_diff_empty.
+
+    Lemma elim_dead_is_bp : 
+      forall fs s used vs vt heap vt' heap', 
+        let result := elim_dead s used in
+        let t := fst result in
+        let used' := snd result in
+        RunsTo fs t (vt, heap) (vt', heap') ->
+        agree_in vs vt used' ->
+        exists vs',
+          RunsTo fs s (vs, heap) (vs', heap') /\
+          agree_in vs' vt' used.
+    Proof.
+      induction s; simpl; intros.
+
+      (* skip *)
+      inversion H; unfold_all; subst.
+      descend.
+      eauto.
+      eauto.
+
+      (* seq *)
+      inversion H; unfold_all; subst.
+      destruct v'; simpl in *.
+      eapply IHs1 in H3; eauto; openhyp.
+      eapply IHs2 in H6; eauto; openhyp.
+      descend.
+      eauto.
+      eauto.
+
+      (* if *)
+      inversion H; unfold_all; subst.
+      simpl in *.
+      eapply IHs1 in H7; eauto; openhyp.
+      descend.
+      eapply RunsToIfTrue.
+      simpl.
+      repeat erewrite (@eval_agree_in _ vs vt) by eauto.
+      eauto.
+      eauto.
+      eauto.
+
+      simpl in *.
+      eapply IHs2 in H7; eauto; openhyp.
+      descend.
+      eapply RunsToIfFalse.
+      simpl.
+      repeat erewrite (@eval_agree_in _ vs vt) by eauto.
+      eauto.
+      eauto.
+      eauto.
+
+      (* while *)
+      eapply while_case in H; eauto.
+
+      Focus 3.
+      (* assign *)
+      openhyp'; simpl in *.
+      inversion H; unfold_all; subst.
+      descend; intuition.
+      econstructor.
+      erewrite eval_agree_in by eauto.
+      simpl in *; eauto.
+
+      inversion H; unfold_all; subst.
+      descend; intuition.
+      econstructor.
+      simpl in *; eauto.
+
+      (* call *)
+      destruct o; simpl in *.
+      inversion H; unfold_all; subst; simpl in *.
+      descend.
+      eapply RunsToCallInternal; simpl in *; eauto.
+      repeat erewrite (@eval_agree_in _ vs vt) by eauto.
+      eauto.
+      repeat erewrite (@eval_agree_in_list _ vs vt) by eauto.
+      eauto.
+      simpl in *.
+      eauto.
+
+      simpl in *.
+      descend.
+      eapply RunsToCallForeign; simpl in *; eauto.
+      repeat erewrite (@eval_agree_in _ vs vt) by eauto.
+      eauto.
+      repeat erewrite (@eval_agree_in_list _ vs vt) by eauto.
+      eauto.
+      simpl in *.
+      eauto.
+
+      inversion H; unfold_all; subst; simpl in *.
+      descend.
+      eapply RunsToCallInternal; simpl in *; eauto.
+      repeat erewrite (@eval_agree_in _ vs vt) by eauto.
+      eauto.
+      repeat erewrite (@eval_agree_in_list _ vs vt) by eauto.
+      eauto.
+      simpl in *.
+      eauto.
+
+      simpl in *.
+      descend.
+      eapply RunsToCallForeign; simpl in *; eauto.
+      repeat erewrite (@eval_agree_in _ vs vt) by eauto.
+      eauto.
+      repeat erewrite (@eval_agree_in_list _ vs vt) by eauto.
+      eauto.
+      simpl in *.
+      eauto.
+
+      (* label *)
+      openhyp'; simpl in *.
+      inversion H; unfold_all; subst.
+      descend; intuition.
+      econstructor; eauto.
+      simpl in *; eauto.
+
+    Qed.
+
+    Lemma elim_dead_is_sp :
+      forall fs s used vs vt heap,
+        let result := elim_dead s used in
+        let t := fst result in
+        let used' := snd result in
+        Safe fs s (vs, heap) ->
+        agree_in vs vt used' ->
+        Safe fs t (vt, heap).
+    Proof.
+      induction s.
+
+      Focus 4.
+      intros.
+      unfold_all.
+      eapply 
+        (Safe_coind 
+           (fun t v =>
+              (exists vs c b used,
+                 let s := While (c) {{b}} in
+                 let result := elim_dead s used in
+                 let s' := fst result in
+                 let used' := snd result in
+                 let vt := fst v in
+                 let heap := snd v in
+                 Safe fs s (vs, heap) /\
+                 agree_in vs vt used' /\
+                 (let s := b in
+                  forall (used : SET) (vs vt : vals) (heap : Heap),
+                    Safe fs s (vs, heap) ->
+                    agree_in vs vt (snd (elim_dead s used)) ->
+                    Safe fs (fst (elim_dead s used)) (vt, heap)
+                 ) /\
+                 t = s') \/
+              Safe fs t v
+        )); [ .. | left; descend; simpl in *; intuition eauto ]; clear; simpl; intros; openhyp.
+
+      (* seq *)
+      intuition.
+
+      inversion H; unfold_all; subst; intuition eauto.
+
+      (* if *)
+      intuition.
+
+      inversion H; subst.
+      unfold_all; openhyp.
+      intuition eauto.
+      right; intuition eauto.
+
+      (* while *)
+      injection H2; intros; subst.
+      inversion H; unfold_all; subst.
+      destruct v; simpl in *.
+      left.
+      repeat split.
+      repeat erewrite (@eval_agree_in _ v x) by eauto.
+      eauto.
+      eauto.
+
+      intros.
+      left.
+      destruct v'; simpl in *.
+      eapply elim_dead_is_bp in H3; eauto; openhyp.
+      descend.
+      4 : eauto.
+      eauto.
+      eauto using subset_trans.
+      eauto.
+
+      simpl in *.
+      right.
+      destruct v; simpl in *.
+      repeat erewrite (@eval_agree_in _ v x) by eauto.
+      eauto.
+
+      inversion H; unfold_all; subst.
+      intuition eauto.
+      right.
+      intuition eauto.
+
+      (* call *)
+      intuition.
+
+      inversion H; unfold_all; subst; eauto.
+
+      left; descend; intuition eauto.
+      right; descend; intuition eauto.
+
+      (* label *)
+      intuition.
+
+      inversion H; unfold_all; subst; intuition eauto.
+
+      (* end of while case *)
+
+      (* skip *)
+      simpl; intros.
+      eauto.
+
+      (* seq *)
+      simpl in *; intros.
+      inversion H; unfold_all; subst.
+      econstructor.
+      eapply IHs1; eauto.
+      intros.
+      destruct v'; simpl in *.
+      eapply elim_dead_is_bp in H1; eauto; openhyp.
+      eapply IHs2; eauto.
+
+      (* if *)
+      simpl in *; intros.
+      inversion H; unfold_all; subst.
+      openhyp.
+      econstructor.
+      left.
+      split.
+      simpl in *.
+      repeat erewrite (@eval_agree_in _ vt vs) by eauto.
+      eauto.
+      eapply IHs1; eauto.
+
+      econstructor.
+      right.
+      split.
+      simpl in *.
+      repeat erewrite (@eval_agree_in _ vt vs) by eauto.
+      eauto.
+      eapply IHs2; eauto.
+
+      Focus 3.
+      (* assign *)
+      simpl; intros; openhyp'; simpl in *; eauto.
+
+      (* call *)
+      simpl; intros.
+      inversion H; unfold_all; subst.
+      econstructor; simpl in *; eauto.
+      repeat erewrite (@eval_agree_in _ vt vs) by eauto.
+      eauto.
+      repeat erewrite (@eval_agree_in_list _ vt vs) by eauto.
+      eauto.
+
+      eapply SafeCallForeign; simpl in *; eauto.
+      repeat erewrite (@eval_agree_in _ vt vs) by eauto.
+      eauto.
+      repeat erewrite (@eval_agree_in_list _ vt vs) by eauto.
+      eauto.
+
+      (* label *)
+      simpl; intros; openhyp'; simpl in *; eauto.
+      inversion_clear H.
+      econstructor; eauto.
+    Qed.  
+
+    Require Import FreeVars.
+
+    Lemma elim_dead_footprint : forall s m, free_vars (fst (elim_dead s m)) <= free_vars s.
+    Proof.
+      induction s; simpl; intros; openhyp'; simpl in *; subset_solver; eauto using subset_trans.
+    Qed.
+
+    Open Scope nat.
+
+    Require Import Depth.
+    Require Import Le.
+    Require Import MaxFacts.
+
+    Hint Extern 0 (le _ _) => progress (simpl; max_solver).
+    Hint Resolve both_le le_n_S.
+
+    Lemma elim_dead_depth : forall s m, depth (fst (elim_dead s m)) <= depth s.
+    Proof.
+      induction s; simpl; intros; openhyp'; simpl in *; max_solver; eauto using le_trans.
+    Qed.
+
+    Definition opt s retvar := fst (elim_dead s (!retvar)).
+
+    Require Import GoodOptimizer.
+
+    Lemma same_agree_in : forall a s, agree_in a a s.
+      unfold agree_in; intros; eauto.
+    Qed.
+
+    Hint Resolve same_agree_in.
+
+    Lemma agree_in_singleton : forall a b x, agree_in a b (!x) -> sel a x = sel b x.
+      intros.
+      eapply H.
+      eapply singleton_iff; eauto.
+    Qed.
+
+    Hint Resolve agree_in_singleton.
+
+    Lemma PreserveRunsTo_opt : PreserveRunsTo opt.
+      unfold PreserveRunsTo, opt; intros.
+      destruct v.
+      destruct v'; simpl in *.
+      eapply elim_dead_is_bp in H; openhyp; eauto.
+    Qed.
+
+    Lemma PreserveSafe_opt : PreserveSafe opt.
+      unfold PreserveSafe, opt; intros.
+      destruct v.
+      eapply elim_dead_is_sp in H; openhyp; eauto.
+    Qed.
+
+    Require Import GetLocalVars.
+    Require Import GetLocalVarsFacts.
+    Import NPeano.Nat.
+
+    Lemma PreserveGoodSize_opt : PreserveGoodSize opt.
+      unfold PreserveGoodSize, opt; intros.
+      eapply goodSize_weaken; eauto.
+      eapply add_le_mono.
+      2 : eapply elim_dead_depth.
+      eapply get_local_vars_cardinal.
+      eapply elim_dead_footprint; eauto.
+    Qed.
+
+    Require Import CompileStmtSpec.
+    Require Import SetoidListFacts.
+    Require Import GeneralTactics2.
+
+    Require Import WellFormed.
+
+    Hint Constructors args_not_too_long.
+
+    Lemma opt_wellformed : forall s m, wellformed s -> wellformed (fst (elim_dead s m)).
+      unfold wellformed.
+      induction s; simpl; intuition; openhyp'; inversion_clear H; simpl in *; eauto.
+    Qed.
+
+    Lemma PreserveSynReq_opt : PreserveSynReq opt.
+      unfold PreserveSynReq, opt; intros.
+      unfold syn_req in *.
+      unfold in_scope in *.
+      openhyp.
+      repeat split; eauto.
+      eapply get_local_vars_subset; eauto.
+      eapply opt_wellformed; eauto.
+    Qed.
+
+    Lemma elim_dead_is_good_optimizer : GoodOptimizer opt.
+      unfold GoodOptimizer.
+      split.
+      eapply PreserveRunsTo_opt.
+      split.
+      eapply PreserveSafe_opt.
+      split.
+      eapply PreserveGoodSize_opt.
+      eapply PreserveSynReq_opt.
+    Qed.
+
+  End TopSection.
+
+End Make.
